theories/Core/Completeness/SubtypingCases.v
@@ -1,0 +1,204 @@
+From Coq Require Import Morphisms_Relations Relation_Definitions.
+
+From McPTS Require Import PtsSignature LibTactics.
+From McPTS.Core Require Import Base.
+From McPTS.Core.Completeness Require Import LogicalRelation SortCases TermStructureCases FunctionCases.
+Import Domain_Notations.
+
+Lemma t {P : PtsSig} {pred_P : PredicativeSig P} : forall s s' r m m', 
+    st_subtyp s s' ->
+    per_sort_elem pred_P s r m m' ->
+    per_sort_elem pred_P s' r m m'.
+Proof.
+  intros.
+  saturate_refl.
+  specialize (ord_st_subtyp pred_P H) as ?.
+  destruct H3; mauto.
+Qed.
+  
+
+Lemma subtyp_refl {P : PtsSig} {pred_P : PredicativeSig P}  : forall Γ M M' s,
+    {{ ⟪ pred_P ⟫ Γ ⊨ M ≈ M' : Sort@s }} ->
+    {{ ⟪ pred_P ⟫ Γ ⊨ M ⊆ M' }}.
+Proof.
+  intros * [env_relΓ].
+  destruct_conjs.
+  eexists_subtyp.
+  intros.
+  saturate_refl.
+  (on_all_hyp: destruct_rel_by_assumption env_relΓ).
+  destruct_by_head (@rel_typ P).
+  invert_rel_typ_body.
+  destruct_by_head (@rel_exp P).
+  unfold per_sort_rec in *.
+  destruct_conjs.
+  handle_per_sort_elem_irrel.
+  do 2 eexists.
+  repeat split; econstructor; mauto 3; econstructor;
+    etransitivity; try eassumption; symmetry; eassumption.
+Qed.
+
+Lemma subtyp_refl_unsorted {P : PtsSig} {pred_P : PredicativeSig P}  : forall Γ M M' s,
+    {{ ⟪ pred_P ⟫ Γ ⊨u M ≈ M' : Sort@s }} ->
+    {{ ⟪ pred_P ⟫ Γ ⊨ M ⊆ M' }}.
+Proof.
+  intros * [env_relΓ]%rel_exp_unsorted_of_typ_inversion1.
+  destruct_conjs.
+  eexists_subtyp.
+  intros.
+  saturate_refl.
+  (on_all_hyp: destruct_rel_by_assumption env_relΓ).
+  destruct_by_head (@rel_typ_unsorted P).
+  destruct_by_head @per_sort.
+  handle_per_sort_elem_irrel.
+  do 2 eexists.
+  repeat split; repeat split; econstructor; mauto 3; econstructor;
+    etransitivity; try eassumption; symmetry; eassumption.
+Qed.
+
+Lemma subtyp_trans {P : PtsSig} {pred_P : PredicativeSig P } : forall Γ M M' M'',
+    {{ ⟪ pred_P ⟫ Γ ⊨ M ⊆ M' }} ->
+    {{ ⟪ pred_P ⟫ Γ ⊨ M' ⊆ M'' }} ->
+    {{ ⟪ pred_P ⟫ Γ ⊨ M ⊆ M'' }}.
+Proof.
+  intros * [env_relΓ [? ?]] [? [? ?]].
+  destruct_conjs.
+  pose env_relΓ.
+  handle_per_ctx_env_irrel.
+  eexists_subtyp.
+  intros.
+  saturate_refl.
+  (on_all_hyp: destruct_rel_by_assumption env_relΓ).
+  destruct_by_head (@rel_typ_unsorted P).
+  destruct_by_head (@rel_exp P).
+  destruct_conjs.
+  handle_per_sort_elem_irrel.
+  do 2 eexists.
+  repeat split; econstructor;
+    eauto using per_sort_elem_cumu.
+  etransitivity;
+    eauto using per_subtyp_sorted_cumu.
+Qed.
+
+#[export]
+Instance subtyp_Transitive {P} {pred_P : PredicativeSig P} Γ : Transitive ((@subtyp_under_ctx P pred_P) Γ).
+Proof. eauto using subtyp_trans. Qed.
+
+Lemma subtyp_sort {P} {pred_P : PredicativeSig P} : forall Γ s1 s2,
+    {{ ⟪ pred_P ⟫ ⊨ Γ }} ->
+    st_subtyp s1 s2 ->
+    {{ ⟪ pred_P ⟫ Γ ⊨ Sort@s1 ⊆ Sort@s2 }}.
+Proof.
+  intros * [env_relΓ] ?.
+  eexists_subtyp.
+  intros.
+  do 2 eexists.
+  repeat split; econstructor; mauto; try econstructor; mauto; try reflexivity.
+Qed.
+
+Lemma subtyp_pi {P} {pred_P : PredicativeSig P} : forall {s1 s2 s3} {r : Ru_pi P s1 s2 s3} Γ A A' B B',
+  {{ ⟪ pred_P ⟫ Γ ⊨u A ≈ A' : Sort@s1 }} ->
+  {{ ⟪ pred_P ⟫ Γ , A@s1 ⊨u B : Sort@s2 }} ->
+  {{ ⟪ pred_P ⟫ Γ , A'@s1 ⊨u B' : Sort@s2 }} ->
+  {{ ⟪ pred_P ⟫ Γ , A'@s1 ⊨ B ⊆ B' }} ->
+  {{ ⟪ pred_P ⟫ Γ ⊨ Π r A B ⊆ Π r A' B' }}.
+Proof.
+  intros * [env_relΓ]%rel_exp_unsorted_of_typ_inversion1 []%rel_exp_unsorted_of_typ_inversion1 []%rel_exp_unsorted_of_typ_inversion1 [? [? ?]].
+  destruct_conjs.
+  handle_per_ctx_env_irrel.
+  invert_per_ctx_envs.
+  match goal with
+  | _: _ <~> cons_per_ctx_env env_relΓ ?x |- _ =>
+      rename x into head_relA'
+  end.
+  handle_per_ctx_env_irrel.
+  eexists_subtyp.
+  intros.
+  saturate_refl.
+  (on_all_hyp: destruct_rel_by_assumption env_relΓ).
+  destruct_by_head @per_sort.
+  handle_per_sort_elem_irrel.
+  (* destruct H0. *)
+  (* destruct_by_head (@rel_exp P). *)
+  (* destruct_conjs. *)
+  
+  assert (forall c c', head_relA' ρ ρ' equiv_ρ_ρ' c c' -> cons_per_ctx_env env_relΓ head_relA' d{{{ ρ ↦ c }}} d{{{ ρ' ↦ c' }}}) as HΓA'
+      by (intros; econstructor; mauto).
+  assert (forall c c', head_rel ρ ρ' equiv_ρ_ρ' c c' -> cons_per_ctx_env env_relΓ head_rel d{{{ ρ ↦ c }}} d{{{ ρ' ↦ c' }}}) as HΓA'0
+      by (intros; econstructor; mauto). 
+
+  (** The proofs for the next two assertions are basically the same *)
+  exvar (relation (domain P))
+    ltac:(fun R => assert ({{ DF Π r a0 ρ B ≈ Π r a ρ' B ∈ per_sort_elem pred_P s3 ↘ R }})).
+  {
+    intros.
+    per_sort_elem_econstructor; [econstructor | | | solve_refl].
+    -  etransitivity; [| symmetry]; mauto.
+    - eapply rel_exp_pi_core; [| reflexivity].
+      intros.
+      assert {{ Dom ρ ↦ c ≈ ρ' ↦ c' ∈ cons_per_ctx_env env_relΓ head_relA' }} as equiv_ρc_ρ'c' by (apply HΓA'; intuition).
+      (on_all_hyp: fun H => destruct (H _ _ equiv_ρc_ρ'c')).
+      destruct_conjs.
+      destruct_by_head @rel_typ_unsorted.
+      destruct_by_head @rel_exp.      
+      econstructor; mauto.
+  }
+  exvar (relation (domain P))
+    ltac:(fun R => assert ({{ DF Π r a0 ρ B' ≈ Π r a ρ' B' ∈ per_sort_elem pred_P s3 ↘ R }})).
+  {
+    per_sort_elem_econstructor; [econstructor | | | solve_refl].
+    - etransitivity; [| symmetry]; mauto.
+    - eapply rel_exp_pi_core; [| reflexivity].
+      intros.
+      assert {{ Dom ρ ↦ c ≈ ρ' ↦ c' ∈ cons_per_ctx_env env_relΓ head_relA' }} as equiv_ρc_ρ'c' by (apply HΓA'; intuition).
+      assert {{ Dom ρ ↦ c ≈ ρ' ↦ c' ∈ cons_per_ctx_env env_relΓ head_rel }} as equiv_ρc_ρ'c'0 by (apply HΓA'0; intuition).
+      simpl in *.
+      (on_all_hyp: fun H => destruct (H _ _ equiv_ρc_ρ'c')).
+      (on_all_hyp: fun H => destruct (H _ _ equiv_ρc_ρ'c'0)).
+      econstructor; mauto.
+  }
+
+  exvar (relation (domain P))
+    ltac:(fun R => assert ({{ DF Π r a3 ρ B ≈ Π r a2 ρ' B ∈ per_sort_elem pred_P s3 ↘ R }})).
+  {
+    intros.
+    per_sort_elem_econstructor; [econstructor | mauto 2 | | solve_refl].
+    - eapply rel_exp_pi_core; [| reflexivity].
+      intros.
+      assert {{ Dom ρ ↦ c ≈ ρ' ↦ c' ∈ cons_per_ctx_env env_relΓ head_relA' }} as equiv_ρc_ρ'c' by (apply HΓA'; intuition).
+      simpl in *.
+      (on_all_hyp: fun H => destruct (H _ _ equiv_ρc_ρ'c')).
+      econstructor; mauto.
+  }
+  exvar (relation (domain P))
+    ltac:(fun R => assert ({{ DF Π r a3 ρ B' ≈ Π r a2 ρ' B' ∈ per_sort_elem pred_P s3 ↘ R }})).
+  {
+    per_sort_elem_econstructor; [econstructor | mauto 2 | | solve_refl].
+    - eapply rel_exp_pi_core; [| reflexivity].
+      intros.
+      assert {{ Dom ρ ↦ c ≈ ρ' ↦ c' ∈ cons_per_ctx_env env_relΓ head_relA' }} as equiv_ρc_ρ'c' by (apply HΓA'; intuition).
+      assert {{ Dom ρ ↦ c ≈ ρ' ↦ c' ∈ cons_per_ctx_env env_relΓ head_rel }} as equiv_ρc_ρ'c'0 by (apply HΓA'0; intuition).
+      simpl in *.
+      (on_all_hyp: fun H => destruct (H _ _ equiv_ρc_ρ'c')).
+      (on_all_hyp: fun H => destruct (H _ _ equiv_ρc_ρ'c'0)).
+      econstructor; mauto.
+  }
+  
+  do 2 eexists.
+  repeat split; econstructor; mauto 2.
+  do 2 econstructor;
+  only 1: mauto;
+  only 3-4: try (saturate_refl; mautosolve 2).
+  - eauto using per_sort_elem_cumu.
+  - intros.
+    assert (cons_per_ctx_env env_relΓ head_relA' d{{{ ρ ↦ c }}} d{{{ ρ' ↦ c' }}}) as equiv_ρc_ρ'c' by (apply HΓA'; intuition).
+    assert (cons_per_ctx_env env_relΓ head_rel d{{{ ρ ↦ c }}} d{{{ ρ' ↦ c' }}}) as equiv_ρc_ρ'c'0 by (apply HΓA'0; intuition).
+    simpl in *.
+    (on_all_hyp: fun H => destruct (H _ _ equiv_ρc_ρ'c')).
+    (on_all_hyp: fun H => destruct (H _ _ equiv_ρc_ρ'c'0)).
+    destruct_conjs.
+    destruct_by_head @rel_mod_eval.
+    destruct H42.
+    handle_per_sort_elem_irrel.
+    mauto using per_subtyp_sorted_cumu.
+Admitted.
